\documentclass{article}
\usepackage{amsmath}
\usepackage{amssymb}
\usepackage[svgnames]{xcolor}
\usepackage{graphicx}
\usepackage{enumitem}
\usepackage{multicol}
\usepackage{graphicx}
\usepackage{color}


\begin{document}
\section{Conditional Independence}

\noindent P(A) = 1st coin flip shows head\\
P(B) = 2nd coin flip shows head\\
P(C) = coin is biased (has two heads)

\begin{table}[htb]
\caption{C=0}
\centering
  \begin{tabular}{ | c | c | c| c | c|}
    \hline
    A & B & $P(A|C)$ & $P(B|C)$ & $P(A,B|C)$ \\ \hline
    0 & 1 & $\frac{1}{2}$ & $\frac{1}{2}$ & $\frac{1}{2}\cdot\frac{1}{2}$ = $\frac{1}{4}$ \\ \hline 
    0 & 0 & $\frac{1}{2}$ & $\frac{1}{2}$ & $\frac{1}{2}\cdot \frac{1}{2}$ = $\frac{1}{4}$ \\ \hline
    1 & 1 & $\frac{1}{2}$ & $\frac{1}{2}$ & $\frac{1}{2}\cdot\frac{1}{2}$ = $\frac{1}{4}$ \\ \hline
    1 & 0 & $\frac{1}{2}$ & $\frac{1}{2}$ & $\frac{1}{2}\cdot\frac{1}{2}$ = $\frac{1}{4}$ \\  \hline
  \end{tabular}
  \end{table}

\begin{table}[htb]
\caption{C=1}
\centering
  \begin{tabular}{ | c | c | c| c | c|}
    \hline
    A & B & $P(A|C)$ & $P(B|C)$ & $P(A,B|C)$ \\ \hline
    0 & 1 &0 &1 & 0 \\ \hline 
    0 & 0 &0 & 0 & 0 \\ \hline
    1 & 1 & 1 & 1 & 1 \\ \hline
    1 & 0 & 1 & 0 & 0 \\  \hline
  \end{tabular}
  \end{table}

\begin{align*}
P(A) &= P(A|C)P(C)+P(A|\overline{C})P(\overline{C}) \\&= \frac{1}{2}\cdot\frac{1}{2} + 1\cdot\frac{1}{2}=\frac{3}{4}\\
P(B) &= P(B|C)P(C)+P(B|\overline{C})P(\overline{C}) \\&= \frac{1}{2}\cdot\frac{1}{2} + 1\cdot\frac{1}{2}=\frac{3}{4}\\
P(A,B) &= P(A, B|C)P(C)+P(A, B|\overline{C})P(\overline{C}) \\&= P(A|C)P(B|C)P(C)+P(A|\overline{C})P(B|\overline{C})P(\overline{C})\\& = \frac{1}{2}\cdot \frac{1}{2}\cdot \frac{1}{2}  + 1\cdot 1\cdot \frac{1}{2}= \frac{5}{8}
\\
P(A)P(B) &= \frac{9}{16} \neq P(A,B) = \frac{5}{8}
\end{align*}

\section{Boy Problem}
	\begin{align*}
		&\frac{p\left(A=b  \wedge B=b  \wedge \left(\left(A=b \wedge A_d = d\right)\vee \left(B=b \wedge B_d = d\right)\right)\right)}{p\left(\left(A=b \wedge A_d = d\right)\vee \left(B=b \wedge B_d = d\right)\right)}\\
		=&\frac{p\left(A=b  \wedge B=b  \wedge \neg\left(A_d =\neg d \wedge B_d = \neg d\right)\right)}{p\left(\neg \left(\neg\left(A=b \wedge A_d = d\right)\wedge \neg\left(B=b \wedge B_d = d\right)\right)\right)}\\
		=&\frac{\frac{1}{2}\frac{1}{2}\left(1-\frac{C-1}{C}\frac{C-1}{C}\right)}{1-\left(1-\frac{1}{2C}\right)^2}\\
		=&\frac{\frac{1}{4}\left(1-\frac{(C-1)^2}{C^2}\right)}{1-\left(1-\frac{1}{2C}\right)^2}\\
		=&\frac{\frac{1}{4}\left(1-\frac{(C^2-2C+1)}{C^2}\right)}{\frac{1}{C}-\frac{1}{4C^2}} \qquad \leftarrow\text{ extend by } \frac{C^2}{C^2} \\
		=&\frac{\frac{1}{4}(2C-1)}{C-\frac{1}{4}}\\
		=& \frac{2C-1}{4C-1}
	\end{align*}

\end{document}
